src/MemCache.v
@@ -22,139 +22,142 @@ Section MemCache.
 
   Variable (st:Type).
 
-  Inductive cache_entry : Type :=
-  | Clean (v:valu) (s:st)
-  | Dirty (v:valu) (s:st)
-  | Invalid (s:st).
+  Inductive cached_val : Type :=
+  | Clean (v:valu)
+  | Dirty (v:valu)
+  | Invalid.
 
-  Definition AssocCache := Map.t cache_entry.
-  Definition cache_add (c:AssocCache) a v s := Map.add a (Clean v s) c.
+  Definition cache_entry : Type := cached_val * st.
 
-  Definition cache_get (c:AssocCache) (a0:addr) : option cache_entry :=
-    Map.find a0 c.
+  Definition AssocCache : Type := Map.t cache_entry.
 
-  Definition cache_dirty (c:AssocCache) (a:addr) v' :=
-    match (Map.find a c) with
-    | Some _ => Map.add a v' c
+  Variable (c:AssocCache).
+
+  Definition cache_get (a:addr) : option cache_entry :=
+    Map.find a c.
+
+  Definition cache_alloc a s :=
+    match cache_get a with
+    | Some _ => c
+    | None => Map.add a (Invalid, s) c
+    end.
+
+  Definition cache_change a (fv: cached_val -> cached_val) (fs: st -> st) :=
+    match cache_get a with
+    | Some (v, s) => Map.add a (fv v, fs s) c
     | None => c
     end.
 
-  Definition cache_add_dirty (c:AssocCache) (a:addr) v' l :=
-    Map.add a (Dirty v' l) c.
+  Definition cache_add a v :=
+    cache_change a (fun _ => v) id.
+
+  Definition cache_dirty a v' :=
+    cache_change a (fun _ => Dirty v') id.
 
   (** Evict a clean address *)
-  Definition cache_evict (c:AssocCache) (a:addr) :=
-    match (Map.find a c) with
-    | Some (Clean _ _) => Map.remove a c
+  Definition cache_evict (a:addr) :=
+    match cache_get a with
+    | Some (Clean _, _) => Map.remove a c
     (* dirty/miss *)
     | _ => c
     end.
 
   (** Change a dirty mapping to a clean one, keeping the same
   value. Intended for use after writeback. *)
-  Definition cache_clean (c:AssocCache) (a:addr) :=
-    match (Map.find a c) with
-    | Some (Dirty v l) => Map.add a (Clean v l) c
-    | _ => c
-    end.
+  Definition cache_clean a :=
+    cache_change a (fun v =>
+                      match v with
+                      | Dirty v => Clean v
+                      | Clean v => Clean v
+                      | Invalid => Invalid
+                      end) id.
 
-  Definition cache_invalidate (c:AssocCache) (a:addr) s :=
-    Map.add a (Invalid s) c.
+  Definition cache_set_state (a:addr) s' :=
+    cache_change a id (fun _ => s').
 
-  Definition cache_set_state (c:AssocCache) (a:addr) s' :=
-    match (Map.find a c) with
-    | Some (Clean v _) => Map.add a (Clean v s') c
-    | Some (Dirty v _) => Map.add a (Dirty v s') c
-    | Some (Invalid _) => Map.add a (Invalid s') c
-    | None => c
-    end.
-
-  Definition cache_val (c:AssocCache) (a:addr) : option valu :=
-    match (Map.find a c) with
-    | Some (Clean v _) => Some v
-    | Some (Dirty v _) => Some v
-    | Some (Invalid _) => None
+  Definition cache_val (a:addr) : option valu :=
+    match cache_get a with
+    | Some (Clean v, _) => Some v
+    | Some (Dirty v, _) => Some v
+    | Some (Invalid, _) => None
     | None => None
     end.
 
-  Definition cache_state (c:AssocCache) a :=
-    match (Map.find a c) with
-    | Some (Clean _ s) => Some s
-    | Some (Dirty _ s) => Some s
-    | Some (Invalid s) => Some s
-    | None => None
+  Definition cache_state a def :=
+    match cache_get a with
+    | Some (_, s) => s
+    | None => def
     end.
 
 End MemCache.
 
-Arguments Invalid {st} s.
+Definition cache_fun st := addr -> cache_entry st.
 
-Definition cache_pred st (c:AssocCache st) (vd:DISK) : DISK_PRED :=
+Definition cache_rep st (c:AssocCache st) (def:st) : cache_fun st :=
+  fun a => match cache_get c a with
+         | Some (v, s) => (v, s)
+         | None => (Invalid, def)
+         end.
+
+Definition cache_fun_state st (f: cache_fun st) a : st :=
+  match f a with
+  | (_, s) => s
+  end.
+
+Definition cache_pred st (c: cache_fun st) (vd:DISK) : DISK_PRED :=
   fun d => forall a,
-      match (cache_get c a) with
-      | Some (Clean v _) => exists rest reader,
+      match c a with
+      | (Clean v, _) => exists rest reader,
                            vd a = Some (Valuset v rest, reader) /\
                            d a = Some (Valuset v rest, reader)
-      | Some (Dirty v' _) => exists rest v reader,
+      | (Dirty v', _) => exists rest v reader,
                            vd a = Some (Valuset v' (v :: rest), reader) /\
                            d a = Some (Valuset v rest, reader)
-      | Some (Invalid _) => vd a = d a
-      | None => vd a = d a
+      | (Invalid, _) => vd a = d a
       end.
 
-(* TODO: replace with map for option *)
-Definition mcache_get_lock (c:AssocCache BusyFlag) a :=
-  match (cache_state c a) with
-  | Some l => l
-  | None => Open
-  end.
+Definition reader_lock_inv (vd: DISK) (c: cache_fun BusyFlagOwner) : Prop :=
+  forall a tid vs v s,
+    vd a = Some (vs, Some tid) ->
+    c a = (v, s) ->
+    s = Owned tid.
 
-Definition gcache_get_lock (c:AssocCache BusyFlagOwner) (a: addr) :=
-  match (cache_state c a) with
-  | Some l => l
-  | None => NoOwner
-  end.
-
-Definition reader_lock_inv : DISK -> AssocCache BusyFlagOwner -> Prop :=
-  fun vd c => (forall a tid vs,
-                vd a = Some (vs, Some tid) ->
-                gcache_get_lock c a = Owned tid).
-
-Inductive cache_addr_eq st st' (st_eq: st -> st' -> Prop) :
-  option (cache_entry st) ->
-  option (cache_entry st') -> Prop :=
-| addr_clean : forall v s s', st_eq s s' -> cache_addr_eq st_eq (Some (Clean v s)) (Some (Clean v s'))
-| addr_dirty : forall v s s', st_eq s s' -> cache_addr_eq st_eq (Some (Dirty v s)) (Some (Dirty v s'))
-| addr_invalid : forall s s', st_eq s s' -> cache_addr_eq st_eq (Some (Invalid s)) (Some (Invalid s'))
-| addr_none : cache_addr_eq st_eq None None.
-
-Hint Constructors cache_addr_eq.
+Definition cache_addr_eq st st' (st_eq: st -> st' -> Prop)
+           (vs: cache_entry st) (vs': cache_entry st') :=
+  forall v s v' s',
+    vs = (v, s) ->
+    vs' = (v', s') ->
+    v = v' /\ st_eq s s'.
 
 Definition cache_eq st st' (st_eq: st -> st' -> Prop)
-  (c:AssocCache st) (c':AssocCache st') :=
-  forall a:addr, cache_addr_eq st_eq (cache_get c a) (cache_get c' a).
+           (c:cache_fun st) (c':cache_fun st') :=
+  forall a, cache_addr_eq st_eq (c a) (c' a).
 
-Ltac replace_cache_vals :=
-  repeat
-    match goal with
-    | [ H: context[cache_get ?c ?a], Heq: cache_get ?c ?a = _ |- _ ] =>
-      replace (cache_get c a) in H
-    | [ Heq: cache_get ?c ?a = _ |- context[cache_get ?c ?a] ] =>
-      replace (cache_get c a)
-    end.
-
-Ltac disk_equalities :=
-  repeat
-    lazymatch goal with
-    | [ a: addr, H: @eq DISK _ _ |- _ ] =>
-      (* this branch pattern may not be useful anymore *)
-      learn H (apply equal_f with a in H);
-        replace_cache_vals
-    | [ |- @eq DISK _ _ ] =>
-      extensionality a'
-    end.
+Definition cache_set st (c: cache_fun st) a ce :=
+  fun a' => if weq a a' then ce else c a'.
 
 Hint Unfold Map.key AddrM.sz : cache_m.
+
+Theorem cache_set_eq : forall st (c: cache_fun st) a ce a',
+    a = a' ->
+    cache_set c a ce a' = ce.
+Proof.
+  unfold cache_set.
+  intros.
+  destruct (weq a a'); congruence.
+Qed.
+
+Theorem cache_set_neq : forall st (c: cache_fun st) a ce a',
+    a <> a' ->
+    cache_set c a ce a' = c a'.
+Proof.
+  unfold cache_set.
+  intros.
+  destruct (weq a a'); congruence.
+Qed.
+
+Hint Rewrite cache_set_eq using (solve [ auto ]) : cache.
+Hint Rewrite cache_set_neq using (solve [ auto ]) : cache.
 
 Lemma weq_same : forall sz a,
     @weq sz a a = left (eq_refl a).
@@ -179,8 +182,6 @@ Ltac distinguish_two_addresses a1 a2 :=
     subst;
     try congruence.
 
-Local Ltac finish := cleanup; eauto.
-
 Ltac distinguish_addresses :=
   try match goal with
   | [ a1 : addr, a2 : addr |- _ ] =>
@@ -194,7 +195,22 @@ Ltac distinguish_addresses :=
     distinguish_two_addresses a1 a2
   end;
   try rewrite weq_same in *;
-  finish.
+  cleanup; eauto.
+
+Ltac single_addr :=
+  lazymatch goal with
+  | [ a: addr, H: forall (_:addr), _ |- _ ] =>
+    lazymatch goal with
+    | [ a: addr, a': addr |- _ ] => fail
+    | _ =>  specialize (H a); destruct_ands
+    end
+  end.
+
+Ltac specific_addrs :=
+  repeat match goal with
+         | [ a: addr, H: forall (_:addr), _ |- _ ] =>
+           learn that (H a)
+         end.
 
 Ltac complete_mem_equalities :=
   try match goal with
@@ -204,141 +220,7 @@ Ltac complete_mem_equalities :=
     learn H' rewrite H in H'
   end.
 
-Hint Unfold cache_pred mem_union : cache.
-
-Section CacheValEquiv.
-
-Variable st:Type.
-Variable c:AssocCache st.
-Variable a:addr.
-
-Ltac t := unfold cache_get, cache_val;
-  intros;
-  now simpl_match.
-
-Lemma cache_val_get_none :
-  cache_get c a = None ->
-  cache_val c a = None.
-Proof. t. Qed.
-
-Lemma cache_val_get_invalid : forall s,
-  cache_get c a = Some (Invalid s) ->
-  cache_val c a = None.
-Proof. t. Qed.
-
-Lemma cache_val_get_none' :
-  cache_val c a = None ->
-  cache_get c a = None \/
-  exists s, cache_get c a = Some (Invalid s).
-Proof.
-  unfold cache_get, cache_val; intros.
-  destruct matches in *; eauto.
-Qed.
-
-Lemma cache_val_get_clean : forall v s,
-  cache_get c a = Some (Clean v s) ->
-  cache_val c a = Some v.
-Proof. t. Qed.
-
-Lemma cache_val_get_dirty : forall v s,
-  cache_get c a = Some (Dirty v s) ->
-  cache_val c a = Some v.
-Proof. t. Qed.
-
-Lemma cache_val_get_some' : forall v,
-  cache_val c a = Some v ->
-  (exists s, cache_get c a = Some (Clean v s)) \/
-  (exists s, cache_get c a = Some (Dirty v s)).
-Proof.
-  unfold cache_get, cache_val; intros.
-    destruct matches in *;
-    match goal with
-    | [ H: Some _ = Some _ |- _ ] => inversion H; subst
-    end; eauto.
-Qed.
-
-End CacheValEquiv.
-
-Hint Resolve cache_val_get_none
-  cache_val_get_invalid
-  cache_val_get_clean
-  cache_val_get_dirty.
-
-Lemma cache_state_as_get : forall st (c:AssocCache st) a,
-    cache_state c a =
-    match cache_get c a with
-    | Some (Clean _ s) => Some s
-    | Some (Dirty _ s) => Some s
-    | Some (Invalid s) => Some s
-    | None => None
-    end.
-Proof.
-  unfold cache_state, cache_get; auto.
-Qed.
-
-Ltac prove_cache_pred :=
-  intros;
-  autounfold with cache_m in *;
-  repeat match goal with
-  | [ |- context[cache_pred] ] =>
-    autounfold with cache; intuition;
-    disk_equalities
-  | [ H_cache_pred: context[cache_pred] |- _ ] =>
-    autounfold with cache in H_cache_pred; intuition;
-    disk_equalities
-  | [ a:addr, H: forall (_:addr), _ |- _ ] =>
-    learn H (specialize (H a);
-              replace_cache_vals)
-  | [ H: cache_val _ _ = None |- _ ] =>
-    apply cache_val_get_none' in H; destruct H
-  | [ H: cache_val _ _ = Some _ |- _ ] =>
-    apply cache_val_get_some' in H; destruct H
-         end;
-  repeat deex;
-  complete_mem_equalities;
-  distinguish_addresses;
-  finish.
-
-Lemma cache_miss_mem_eq : forall st (c:AssocCache st) vd a d,
-    cache_pred c vd d ->
-    cache_val c a = None ->
-    vd a = d a.
-Proof.
-  prove_cache_pred.
-Qed.
-
-Lemma cache_pred_except : forall st (c:AssocCache st) vd m a,
-    cache_val c a = None ->
-    cache_pred c vd m ->
-    cache_pred c (mem_except vd a) (mem_except m a).
-Proof.
-  unfold mem_except.
-  prove_cache_pred.
-Qed.
-
-Lemma cache_pred_address : forall st (c:AssocCache st) vd a v,
-    cache_val c a = None ->
-    vd a = Some v ->
-    cache_pred c vd =p=>
-cache_pred c (mem_except vd a) * a |-> v.
-Proof.
-  unfold pimpl.
-  intros.
-  unfold_sep_star.
-  exists (mem_except m a).
-  exists (fun a' => if weq a' a then Some v else None).
-  unfold mem_except.
-  prove_cache_pred; destruct matches.
-  unfold mem_disjoint; intro; repeat deex.
-  destruct matches in *.
-
-  unfold mem_disjoint; intro; repeat deex.
-  destruct matches in *.
-
-  unfold ptsto; intuition; distinguish_addresses.
-
-  unfold ptsto; intuition; distinguish_addresses.
-Qed.
+Hint Unfold cache_pred : cache.
 
 Section CacheGetFacts.
 
@@ -376,8 +258,50 @@ Proof.
   apply MapFacts.remove_neq_o; auto.
 Qed.
 
-Hint Unfold cache_get cache_add cache_add_dirty
-            cache_evict cache_clean cache_invalidate cache_set_state : cache_get.
+Lemma cache_rep_get : forall st (c:AssocCache st) def a v s,
+    cache_get c a = Some (v, s) ->
+    cache_rep c def a = (v, s).
+Proof.
+  unfold cache_rep; intros; now simpl_match.
+Qed.
+
+Lemma cache_rep_get_def : forall st (c:AssocCache st) def a,
+    cache_get c a = None ->
+    cache_rep c def a = (Invalid, def).
+Proof.
+  unfold cache_rep; intros; now simpl_match.
+Qed.
+
+Lemma cache_rep_change_get : forall st (c:AssocCache st) def a
+                               v s fv fs,
+    cache_get c a = Some (v, s) ->
+    cache_rep (cache_change c a fv fs) def a = (fv v, fs s).
+Proof.
+  unfold cache_rep, cache_change; intros; simpl_match.
+  cbn; rewrite map_raw_add_eq_o by auto; auto.
+Qed.
+
+Lemma cache_rep_change_get_def : forall st (c:AssocCache st) def a
+                               fv fs,
+    cache_get c a = None ->
+    cache_rep (cache_change c a fv fs) def a = (Invalid, def).
+Proof.
+  unfold cache_rep, cache_change; intros; simpl_match.
+  rewrite H; auto.
+Qed.
+
+Lemma cache_rep_change_get_neq : forall st (c:AssocCache st) def a a' fv fs,
+    a <> a' ->
+    cache_rep (cache_change c a fv fs) def a' = cache_rep c def a'.
+Proof.
+  unfold cache_rep, cache_change; intros.
+  case_eq (cache_get c a); intros; auto.
+  destruct c0; cbn.
+  rewrite map_raw_add_neq_o by auto; auto.
+Qed.
+
+Hint Unfold cache_get cache_add
+            cache_evict cache_clean cache_set_state : cache_get.
 
 Ltac t := autounfold with cache_get;
   intuition;
@@ -386,149 +310,9 @@ Ltac t := autounfold with cache_get;
   try congruence;
   auto.
 
-Lemma cache_get_eq : forall st (c:AssocCache st) a v s,
-    cache_get (cache_add c a v s) a = Some (Clean v s).
-Proof.
-  t.
-Qed.
-
-Lemma cache_get_dirty_eq : forall st (c:AssocCache st) a v s,
-    cache_get (cache_add_dirty c a v s) a = Some (Dirty v s).
-Proof.
-  t.
-Qed.
-
-Lemma cache_get_dirty_neq : forall st (c:AssocCache st) a a' v s,
-    a <> a' ->
-    cache_get (cache_add_dirty c a v s) a' = cache_get c a'.
-Proof.
-  t.
-Qed.
-
-Lemma cache_get_neq : forall st (c:AssocCache st) a a' v s,
-    a <> a' ->
-    cache_get (cache_add c a v s) a' = cache_get c a'.
-Proof.
-  t.
-Qed.
-
-Lemma cache_invalidate_get : forall st (c:AssocCache st) a l,
-  cache_state (cache_invalidate c a l) a = Some l.
-Proof.
-  intros.
-  rewrite cache_state_as_get.
-  t.
-Qed.
-
-Lemma cache_invalidate_get_other : forall st (c:AssocCache st) a a' l,
-  a <> a' ->
-  cache_get (cache_invalidate c a l) a' = cache_get c a'.
-Proof.
-  t.
-Qed.
-
-Lemma cache_set_state_get : forall st (c:AssocCache st) a l,
-  cache_get (cache_set_state c a l) a = match cache_get c a with
-  | Some (Clean v _) => Some (Clean v l)
-  | Some (Dirty v _) => Some (Dirty v l)
-  | Some (Invalid _) => Some (Invalid l)
-  | None => None
-  end.
-Proof.
-  t.
-Qed.
-
-Lemma cache_set_state_get_other : forall st (c:AssocCache st) a a' l,
-  a <> a' ->
-  cache_get (cache_set_state c a l) a' = cache_get c a'.
-Proof.
-  t.
-Qed.
-
-Lemma cache_add_invalidate : forall st (c:AssocCache st) a l v l' a',
-  cache_get (cache_add (cache_invalidate c a l) a v l') a' =
-  cache_get (cache_add c a v l') a'.
-Proof.
-  intros.
-  destruct (weq a a'); t.
-Qed.
-
-Lemma cache_evict_get : forall st (c:AssocCache st) v a s,
-  cache_get c a = Some (Clean v s) ->
-  cache_get (cache_evict c a) a = None.
-Proof.
-  t.
-Qed.
-
-Lemma cache_evict_get_other : forall st (c:AssocCache st) a a',
-  a <> a' ->
-  cache_get (cache_evict c a) a' = cache_get c a'.
-Proof.
-  t.
-Qed.
-
-Lemma cache_remove_get : forall st (c:AssocCache st) a,
-  cache_get (Map.remove a c) a = None.
-Proof.
-  t.
-Qed.
-
-Lemma cache_remove_get_other : forall st (c:AssocCache st) a a',
-  a <> a' ->
-  cache_get (Map.remove a c) a' = cache_get c a'.
-Proof.
-  t.
-Qed.
-
-Lemma cache_clean_clean_noop : forall st (c:AssocCache st) a v s,
-    cache_get c a = Some (Clean v s) ->
-    cache_clean c a = c.
-Proof.
-  t.
-Qed.
-
-Lemma cache_get_add_clean : forall st (c:AssocCache st) a v s,
-    cache_get (cache_add c a v s) a = Some (Clean v s).
-Proof.
-  t.
-Qed.
-
-Lemma cache_get_add_other : forall st (c:AssocCache st) a a' v s,
-    a <> a' ->
-    cache_get (cache_add c a v s) a' = cache_get c a'.
-Proof.
-  t.
-Qed.
-
-Lemma cache_get_remove_eq : forall st (c:AssocCache st) a,
-    cache_get (Map.remove a c) a = None.
-Proof.
-  t.
-Qed.
-
-Lemma cache_get_remove_neq : forall st (c:AssocCache st) a a',
-    a <> a' ->
-    cache_get (Map.remove a c) a' = cache_get c a'.
-Proof.
-  t.
-Qed.
-
-Lemma cache_get_clean_neq : forall st (c:AssocCache st) a a',
-    a <> a' ->
-    cache_get (cache_clean c a) a' = cache_get c a'.
-Proof.
-  t.
-Qed.
-
-Lemma cache_get_dirty_clean : forall st (c:AssocCache st) a v s,
-  cache_get c a = Some (Dirty v s) ->
-  cache_get (cache_clean c a) a = Some (Clean v s).
-Proof.
-  t.
-Qed.
-
 End CacheGetFacts.
 
+(*
 Hint Rewrite cache_get_eq cache_get_dirty_eq : cache.
 Hint Rewrite cache_get_dirty_neq cache_get_neq using (now eauto) : cache.
 Hint Rewrite cache_remove_get : cache.
@@ -545,114 +329,62 @@ Hint Rewrite cache_get_remove_eq : cache.
 Hint Rewrite cache_get_remove_neq using (now auto) : cache.
 Hint Rewrite cache_get_clean_neq using (now auto) : cache.
 Hint Rewrite cache_get_dirty_clean using (now auto) : cache.
-Hint Rewrite map_raw_add_eq_o using (now auto): cache.
-Hint Rewrite map_raw_add_neq_o using (now auto): cache.
-Hint Rewrite map_raw_remove_eq_o using (now auto): cache.
-Hint Rewrite map_raw_remove_neq_o using (now auto): cache.
+*)
+Hint Rewrite map_raw_add_eq_o using (solve [ auto ]): cache.
+Hint Rewrite map_raw_add_neq_o using (solve [ auto ]): cache.
+Hint Rewrite map_raw_remove_eq_o using (solve [ auto ]): cache.
+Hint Rewrite map_raw_remove_neq_o using (solve [ auto ]): cache.
+Hint Rewrite cache_rep_get using (solve [ auto ]) : cache.
+Hint Rewrite cache_rep_get_def using (solve [ auto ]) : cache.
+Hint Rewrite cache_rep_change_get using (solve [ auto ]) : cache.
+Hint Rewrite cache_rep_change_get_def using (solve [ auto ]) : cache.
+Hint Rewrite cache_rep_change_get_neq using (solve [ auto ]) : cache.
 
+(* TODO: make this tactic more local *)
 Ltac case_cache_val' c a :=
   case_eq (cache_get c a); intros;
   try lazymatch goal with
       | [ ce: cache_entry _ |- _ ] =>
         destruct ce
-      end;
-  replace_cache_vals;
+    end;
+  try lazymatch goal with
+    | [ cv: cached_val |- _ ] =>
+      destruct cv
+    end;
+  try replace (cache_get c a) in *;
   (* especially to remove impossible cases *)
   try congruence.
 
 Section CacheEqPreserved.
 
 Variable st:Type.
-Variable c:AssocCache st.
+Variable c:cache_fun st.
 Variable st':Type.
-Variable c':AssocCache st'.
+Variable c':cache_fun st'.
 
 Remark cache_eq_refl :
   cache_eq eq c c.
 Proof.
-  unfold cache_eq; intuition.
-  case_cache_val' c a; eauto.
+  unfold cache_eq, cache_addr_eq; intuition; congruence.
 Qed.
 
-Theorem cache_eq_add : forall st_eq (a:addr) v s s',
+Theorem cache_eq_set : forall st_eq (a:addr) v s s',
   cache_eq st_eq c c' ->
   st_eq s s' ->
-  cache_eq st_eq (cache_add c a v s) (cache_add c' a v s').
+  cache_eq st_eq (cache_set c a (v, s)) (cache_set c' a (v, s')).
 Proof.
-  unfold cache_eq; intuition;
+  unfold cache_eq, cache_addr_eq; intros;
     match goal with
     | [ H: forall (_:addr), _, a:addr |- _ ] =>
       specialize (H a); unfold cache_val, cache_state in H
-    end; intuition.
+    end.
 
   distinguish_addresses;
-    repeat rewrite map_raw_add_neq_o by auto;
-    repeat rewrite map_raw_add_eq_o by auto;
-    auto.
-Qed.
-
-Theorem cache_eq_invalidate : forall st_eq (a:addr) s s',
-  cache_eq st_eq c c' ->
-  st_eq s s' ->
-  cache_eq st_eq (cache_invalidate c a s) (cache_invalidate c' a s').
-Proof.
-  unfold cache_eq; intuition;
-    match goal with
-    | [ H: forall (_:addr), _, a:addr |- _ ] =>
-      specialize (H a); unfold cache_val, cache_state in H
-    end; intuition.
-
-  distinguish_addresses;
-    repeat rewrite map_raw_add_neq_o by auto;
-    repeat rewrite map_raw_add_eq_o by auto;
-    auto.
-Qed.
-
-Theorem cache_eq_lock : forall st_eq (a:addr) s s',
-  cache_eq st_eq c c' ->
-  st_eq s s' ->
-  cache_eq st_eq (cache_set_state c a s) (cache_set_state c' a s').
-Proof.
-  unfold cache_eq; intuition;
-    match goal with
-    | [ H: forall (_:addr), _, a:addr |- _ ] =>
-      specialize (H a); unfold cache_val, cache_state in H
-    end; intuition.
-
-  distinguish_addresses;
-    autorewrite with cache;
-    auto.
-  inversion H; eauto.
+    autorewrite with cache in *;
+    repeat inv_prod; auto.
 Qed.
 
 End CacheEqPreserved.
-
-Ltac rewrite_cache_get :=
-  repeat match goal with
-         | [ H: context[cache_get (cache_evict ?c ?a) ?a],
-             H': cache_get ?c ?a = Some (false, ?v) |- _ ] =>
-           rewrite (cache_evict_get c v a H') in H
-         end;
-  autorewrite with cache in *.
-
-Theorem cache_pred_eq_disk : forall st (c:AssocCache st) vd d a v l,
-    cache_get c a = Some (Clean v l) ->
-    cache_pred c vd d ->
-    exists rest reader, d a = Some (Valuset v rest, reader).
-Proof.
-  prove_cache_pred.
-Qed.
-
-Ltac learn_disk_val :=
-  lazymatch goal with
-  | [ Hget: cache_get ?c ?a = Some (Clean ?v _),
-            Hpred: cache_pred ?c ?vd ?d |- _ ] =>
-    try lazymatch goal with
-    | [ H: d a = Some (Valuset v _) |- _ ] => fail 1 "already did that"
-    end;
-      let rest := fresh "rest" in
-      edestruct (cache_pred_eq_disk a Hget Hpred) as [rest ?]
-  end.
 
 Ltac case_cache_val :=
   lazymatch goal with
@@ -672,61 +404,131 @@ Ltac case_cache_val :=
     case_cache_val' c a
   end.
 
-Lemma cache_pred_clean : forall st (c:AssocCache st) vd rest a v l reader,
-    cache_get c a = Some (Clean v l) ->
+Theorem cache_pred_eq_disk : forall st (c:cache_fun st) vd d a v l,
+    c a = (Clean v, l) ->
+    cache_pred c vd d ->
+    exists rest reader, d a = Some (Valuset v rest, reader).
+Proof.
+  unfold cache_pred; intros;
+  single_addr; simpl_match; repeat deex.
+  eauto.
+Qed.
+
+Ltac learn_disk_val :=
+  lazymatch goal with
+  | [ Hget: ?c ?a = (Clean ?v, _),
+            Hpred: cache_pred ?c ?vd ?d |- _ ] =>
+    try lazymatch goal with
+      | [ H: d a = Some (Valuset v _) |- _ ] => fail 1 "already did that"
+      end;
+      let rest := fresh "rest" in
+      edestruct (cache_pred_eq_disk a Hget Hpred) as [rest ?]
+  end.
+
+Lemma cache_pred_miss : forall st (c:cache_fun st) l vd a v rest reader,
+    c a = (Invalid, l) ->
     vd a = Some (Valuset v rest, reader) ->
     cache_pred c vd =p=>
-cache_pred (Map.remove a c) (mem_except vd a) * a |-> (Valuset v rest, reader).
+cache_pred c (mem_except vd a) * a |-> (Valuset v rest, reader).
+Proof.
+  unfold cache_pred, pimpl; intros.
+  unfold_sep_star.
+  exists (mem_except m a).
+  exists (fun a' => if weq a' a then Some (Valuset v rest, reader) else None).
+  unfold mem_union, mem_except.
+  pose proof (H1 a); simpl_match.
+  intuition.
+  extensionality a'.
+  distinguish_addresses.
+  destruct (m a'); now auto.
+  unfold mem_disjoint; intro; repeat deex; now distinguish_addresses.
+  distinguish_addresses.
+  apply H1.
+  unfold ptsto.
+  intuition; distinguish_addresses.
+Qed.
+
+Lemma union_ptsto_to_upd : forall AT AEQ V (m1 m2: @mem AT AEQ V) a v,
+    mem_disjoint m1 m2 ->
+    (a |-> v)%pred m2 ->
+    mem_union m1 m2 = upd m1 a v.
+Proof.
+  unfold ptsto, mem_disjoint, mem_union; intuition.
+  extensionality a'; destruct (AEQ a a'); subst;
+  autorewrite with upd.
+  case_eq (m1 a'); intros; auto.
+  exfalso; eapply H; eauto.
+  erewrite H2; eauto.
+  destruct (m1 a'); auto.
+Qed.
+
+Lemma cache_pred_miss' : forall st (c:cache_fun st) l vd a v rest reader,
+    vd a = Some (Valuset v rest, reader) ->
+    c a = (Invalid, l) ->
+    cache_pred c (mem_except vd a) * a |-> (Valuset v rest, reader) =p=>
+cache_pred c vd.
+Proof.
+  unfold cache_pred, pimpl; intros.
+  unfold_sep_star in H1; repeat deex.
+  erewrite union_ptsto_to_upd; eauto.
+  pose proof (H3 a); simpl_match.
+  pose proof (H3 a0).
+  unfold mem_except in *.
+  rewrite weq_same in *.
+  distinguish_addresses; autorewrite with upd; auto.
+Qed.
+
+Lemma cache_pred_clean : forall st (c:cache_fun st) def vd rest a v l reader,
+    vd a = Some (Valuset v rest, reader) ->
+    c a = (Clean v, l) ->
+    cache_pred c vd =p=>
+cache_pred (cache_set c a (Invalid, def)) (mem_except vd a) * a |-> (Valuset v rest, reader).
 Proof.
   unfold pimpl.
   intros.
   unfold_sep_star.
-  learn_disk_val.
+  learn_disk_val; deex.
 
   exists (mem_except m a).
-  exists (fun a' => if weq a' a then Some (Valuset v rest, reader) else None).
+  exists (fun a' => if weq a' a then Some (Valuset v rest0, reader0) else None).
   unfold mem_except.
   intuition.
-  - unfold mem_union; apply functional_extensionality; intro a'.
-    prove_cache_pred; replace_cache_vals; eauto.
-    destruct matches.
+  - unfold mem_union; extensionality a'.
+    distinguish_addresses; auto.
+    destruct (m a'); auto.
   - unfold mem_disjoint; intro; repeat deex.
-    prove_cache_pred; replace_cache_vals; eauto.
-  - prove_cache_pred; destruct matches in *;
-      rewrite_cache_get; finish.
+    distinguish_addresses.
+  - unfold cache_pred in *; intros; distinguish_addresses;
+    autorewrite with cache; auto.
+    apply H1.
   - unfold ptsto; intuition; distinguish_addresses.
+    unfold const, wr_set in *.
+    unfold cache_pred in *; single_addr; simpl_match; repeat deex.
+    congruence.
 Qed.
 
-Lemma cache_pred_clean' : forall st (c:AssocCache st) vd a rest v l reader,
-    cache_get c a = Some (Clean v l) ->
+Lemma cache_pred_clean' : forall st (c:cache_fun st) def vd a rest v l reader,
+    c a = (Clean v, l) ->
     vd a = Some (Valuset v rest, reader) ->
-    (cache_pred (Map.remove a c) (mem_except vd a) * a |-> (Valuset v rest, reader)) =p=>
+    (cache_pred (cache_set c a (Invalid, def)) (mem_except vd a) * a |-> (Valuset v rest, reader)) =p=>
 cache_pred c vd.
 Proof.
   unfold pimpl, mem_except.
   intros.
   unfold_sep_star in H1.
   repeat deex.
-  unfold ptsto in *; intuition.
-  prove_cache_pred;
-    rewrite_cache_get; disk_equalities; distinguish_addresses; finish.
-
-  case_cache_val;
-    destruct matches;
-    subst;
-    repeat deex;
-    repeat match goal with
-           | [ |- exists _, _ ] => eexists
-           end; intuition eauto;
-           fold wr_set in *;
-           try congruence.
+  erewrite union_ptsto_to_upd; eauto.
+  unfold cache_pred; intros.
+  pose proof (H3 a0).
+  distinguish_addresses; autorewrite with cache upd in *;
+  repeat simpl_match; eauto.
 Qed.
 
-Lemma cache_pred_dirty : forall st (c:AssocCache st) vd a v v' l rest reader,
-    cache_get c a = Some (Dirty v' l) ->
+Lemma cache_pred_dirty : forall st (c:cache_fun st) def vd a v v' l rest reader,
+    c a = (Dirty v', l) ->
     vd a = Some (Valuset v' (v :: rest), reader) ->
     cache_pred c vd =p=>
-    cache_pred (Map.remove a c) (mem_except vd a) *
+    cache_pred (cache_set c a (Invalid, def)) (mem_except vd a) *
       a |-> (Valuset v rest, reader).
 Proof.
   unfold pimpl.
@@ -735,60 +537,64 @@ Proof.
   exists (mem_except m a).
   exists (fun a' => if weq a' a then Some (Valuset v rest, reader) else None).
   unfold mem_except, mem_union, mem_disjoint, ptsto.
-  intuition;
-    prove_cache_pred; replace_cache_vals;
-    try solve [ destruct matches ];
-    rewrite_cache_get; finish.
+  rewrite weq_same.
+  intuition.
+  extensionality a'; distinguish_addresses.
+  pose proof (H1 a); simpl_match; repeat deex.
+  congruence.
+  destruct (m a'); auto.
+  repeat deex.
+  distinguish_addresses.
+
+  unfold cache_pred; intros; distinguish_addresses;
+  autorewrite with cache; auto.
+  apply H1.
+
+  unfold const, wr_set.
+  destruct (weq a' a); try congruence.
 Qed.
 
-Lemma cache_pred_dirty' : forall st (c:AssocCache st) vd a v v' l rest reader,
-    cache_get c a = Some (Dirty v' l) ->
+Lemma cache_pred_dirty' : forall st (c:cache_fun st) def vd a v v' l rest reader,
+    c a = (Dirty v', l) ->
     vd a = Some (Valuset v' (v :: rest), reader) ->
-    cache_pred (Map.remove a c) (mem_except vd a) *
+    cache_pred (cache_set c a (Invalid, def)) (mem_except vd a) *
     a |-> (Valuset v rest, reader) =p=> cache_pred c vd.
 Proof.
   unfold pimpl, mem_except.
   intros.
   unfold_sep_star in H1.
   repeat deex.
-  unfold ptsto in *; intuition.
-  prove_cache_pred; distinguish_addresses;
-  rewrite_cache_get; disk_equalities; distinguish_addresses; finish.
-
-  case_cache_val;
-    destruct matches;
-    subst;
-    repeat deex;
-    repeat match goal with
-    | [ |- exists _, _ ] => eexists
-           end; intuition eauto;
-           fold wr_set in *;
-           try congruence.
+  erewrite union_ptsto_to_upd; eauto.
+  unfold cache_pred; intros.
+  pose proof (H3 a0).
+  distinguish_addresses; autorewrite with cache upd in *;
+  repeat simpl_match; eauto.
 Qed.
 
-Lemma cache_pred_clean_val :  forall st (c:AssocCache st) vd d a v l,
+Lemma cache_pred_clean_val :  forall st (c:cache_fun st) vd d a v l,
     cache_pred c vd d ->
-    cache_get c a = Some (Clean v l) ->
+    c a = (Clean v, l) ->
     exists rest reader, vd a = Some (Valuset v rest, reader) /\
                    d a = Some (Valuset v rest, reader).
 Proof.
-  prove_cache_pred.
+  unfold cache_pred; intros; single_addr; simpl_match; repeat deex; eauto.
 Qed.
 
-Lemma cache_pred_dirty_val :  forall st (c:AssocCache st) vd d a v l,
+Lemma cache_pred_dirty_val :  forall st (c:cache_fun st) vd d a v l,
     cache_pred c vd d ->
-    cache_get c a = Some (Dirty v l) ->
+    c a = (Dirty v, l) ->
     exists v' rest reader,
       vd a = Some (Valuset v (v' :: rest), reader) /\
       d a = Some (Valuset v' rest, reader).
 Proof.
-  prove_cache_pred.
+  unfold cache_pred; intros; single_addr; simpl_match; repeat deex; eauto.
 Qed.
 
 Section CachePredStability.
 
 Hint Rewrite upd_eq upd_ne using (now auto) : cache.
 
+(*
 Lemma cache_pred_same_cache : forall st (c:AssocCache st) vd d c',
   cache_pred c vd d ->
   (forall a, cache_get c' a = cache_get c a) ->
@@ -1005,59 +811,26 @@ Proof.
     try congruence.
 Qed.
 
+*)
+
 End CachePredStability.
+
 
 Section ReaderLockStability.
 
-  Lemma gcache_get_lock_add : forall c a a' v l,
-    a <> a' ->
-    gcache_get_lock (cache_add c a v l) a' =
-    gcache_get_lock c a'.
-  Proof.
-    unfold gcache_get_lock; intros.
-    repeat rewrite cache_state_as_get;
-      autorewrite with cache;
-      reflexivity.
-  Qed.
-
-  Lemma gcache_get_lock_invalidate : forall c a a' l,
-    a <> a' ->
-    gcache_get_lock (cache_invalidate c a l) a' =
-    gcache_get_lock c a'.
-  Proof.
-    unfold gcache_get_lock; intros.
-    repeat rewrite cache_state_as_get;
-      autorewrite with cache.
-      reflexivity.
-  Qed.
-
-  Theorem reader_lock_add_no_reader : forall vd a c v vs l,
+  Theorem reader_lock_add_no_reader : forall vd a c ce vs,
     vd a = Some (vs, None) ->
     reader_lock_inv vd c ->
-    reader_lock_inv vd (cache_add c a v l).
+    reader_lock_inv vd (cache_set c a ce).
   Proof.
     unfold reader_lock_inv.
     intuition.
-    distinguish_two_addresses a a0.
-    rewrite gcache_get_lock_add by (now auto).
-    eauto.
+    distinguish_addresses; autorewrite with cache in *; eauto.
   Qed.
 
-  Lemma reader_lock_invalidate : forall vd a c vs l,
-      vd a = Some (vs, None) ->
+  Lemma reader_lock_add_reader : forall vd a v vs tid c,
       reader_lock_inv vd c ->
-      reader_lock_inv vd (cache_invalidate c a l).
-  Proof.
-    unfold reader_lock_inv.
-    intros.
-    distinguish_addresses.
-    rewrite gcache_get_lock_invalidate by (now auto).
-    eauto.
-  Qed.
-
-  Lemma reader_lock_add_reader : forall vd a vs tid c,
-      reader_lock_inv vd c ->
-      gcache_get_lock c a = Owned tid ->
+      c a = (v, Owned tid) ->
       reader_lock_inv (upd vd a (vs, Some tid)) c.
   Proof.
     unfold reader_lock_inv.
@@ -1078,16 +851,16 @@ Section ReaderLockStability.
 
 End ReaderLockStability.
 
-Theorem cache_pred_same_virt_disk : forall st (c:AssocCache st) vd vd' d,
+Theorem cache_pred_same_virt_disk : forall st (c:cache_fun st) vd vd' d,
     cache_pred c vd d ->
     cache_pred c vd' d ->
     vd = vd'.
 Proof.
-  prove_cache_pred.
-  destruct matches in *; repeat deex; finish.
+  unfold cache_pred; intros; extensionality a; repeat single_addr.
+  destruct matches in *; repeat deex; congruence.
 Qed.
 
-Theorem cache_pred_same_virt_disk_eq : forall st (c:AssocCache st) c' vd vd' d d',
+Theorem cache_pred_same_virt_disk_eq : forall st (c:cache_fun st) c' vd vd' d d',
     c = c' ->
     d = d' ->
     cache_pred c vd d ->
@@ -1098,16 +871,16 @@ Proof.
   eauto using cache_pred_same_virt_disk.
 Qed.
 
-Theorem cache_pred_same_disk : forall st (c:AssocCache st) vd d d',
+Theorem cache_pred_same_disk : forall st (c:cache_fun st) vd d d',
     cache_pred c vd d ->
     cache_pred c vd d' ->
     d = d'.
 Proof.
-  prove_cache_pred.
-  destruct matches in *; repeat deex; finish.
+  unfold cache_pred; intros; extensionality a; repeat single_addr.
+  destruct matches in *; repeat deex; congruence.
 Qed.
 
-Theorem cache_pred_same_disk_eq : forall st (c:AssocCache st) c' vd vd' d d',
+Theorem cache_pred_same_disk_eq : forall st (c:cache_fun st) c' vd vd' d d',
     cache_pred c vd d ->
     cache_pred c' vd' d' ->
     c = c' ->
@@ -1118,24 +891,27 @@ Proof.
   eauto using cache_pred_same_disk.
 Qed.
 
-Lemma cache_get_vd_clean : forall st (c:AssocCache st) d vd a v rest v' l reader,
+Lemma cache_get_vd_clean : forall st (c:cache_fun st) d vd a v rest v' l reader,
   cache_pred c vd d ->
   vd a = Some (Valuset v rest, reader) ->
-  cache_get c a = Some (Clean v' l) ->
+  c a = (Clean v', l) ->
   v' = v.
 Proof.
-  prove_cache_pred.
+  unfold cache_pred; intros; single_addr; simpl_match.
+  repeat deex; congruence.
 Qed.
 
-Lemma cache_get_vd_dirty : forall st (c:AssocCache st) d vd a v rest v' l reader,
+Lemma cache_get_vd_dirty : forall st (c:cache_fun st) d vd a v rest v' l reader,
   cache_pred c vd d ->
   vd a = Some (Valuset v rest, reader) ->
-  cache_get c a = Some (Dirty v' l) ->
+  c a = (Dirty v', l) ->
   v' = v.
 Proof.
-  prove_cache_pred.
+  unfold cache_pred; intros; single_addr; simpl_match.
+  repeat deex; congruence.
 Qed.
 
+(*
 Lemma cache_pred_same_sectors : forall st (c:AssocCache st) vd d,
     cache_pred c vd d ->
     same_domain d vd.
@@ -1170,7 +946,6 @@ Proof.
   autorewrite with upd in *;
   auto; congruence.
 Qed.
-
-
+*)
 
 Hint Opaque cache_pred.
